src/kemedhoc/Impl.KEMEDHOC.Core.Msg3.Aux.Misc.fst
@@ -1,0 +1,219 @@
+module Impl.KEMEDHOC.Core.Msg3.Aux.Misc
+
+(*LowStar related modules*)
+open Lib.ByteBuffer
+open Lib.IntTypes
+open Lib.Buffer
+
+(*HACL Random lib*)
+open Lib.RandomBuffer.System
+module HACLRandom = Lib.RandomSequence
+
+module B = LowStar.Buffer
+module ST = FStar.HyperStack.ST
+module HS = FStar.HyperStack
+module S = FStar.Seq
+module Seq = Lib.Sequence
+
+(*Specification modules*)
+module Spec = Spec.KEMEDHOC.Core
+
+module FBytes = FStar.Bytes
+
+module SpecCrypto = Spec.KEMEDHOC.CryptoPrimitives
+module SpecParser = Spec.KEMEDHOC.Parser
+module SpecTH = Spec.KEMEDHOC.TranscriptHash
+module SpecKS = Spec.KEMEDHOC.KeySchedule
+
+module SpecEdhocSerd = Spec.EDHOC.Serialization
+
+module TypeEdhoc = TypeHelper.EDHOC
+
+(*EDHOC utilities*)
+open Impl.EDHOC.Utilities
+
+(*KEMEDHOC utilities*)
+open Impl.KEMEDHOC.Types
+open Impl.KEMEDHOC.CryptoPrimitives
+open Impl.KEMEDHOC.KeySchedule
+open Impl.KEMEDHOC.Parser
+open Impl.KEMEDHOC.Ciphertext
+open Impl.KEMEDHOC.TranscriptHash
+open Impl.KEMEDHOC.Core
+open Impl.KEMEDHOC.Core.Utilities
+open Impl.KEMEDHOC.Core.Msg3.Aux
+open Spec.KEMEDHOC.Base.Definitions
+
+module AuxMsg2 = Impl.KEMEDHOC.Core.Msg2.Aux
+
+val responder_process_msg3_decrypt_msg3:
+  #kcs: supportedKemCipherSuite
+  -> rs: party_state_m kcs
+  -> hs: handshake_state_m kcs
+  -> p2: plaintext2 kcs
+  -> msg3: message3 kcs
+  -> p3: plaintext3 kcs
+  -> ST.Stack c_response
+  (requires fun h0 ->
+    is_party_state_eph_est_m h0 rs
+    /\ is_valid_handshake_state_m h0 hs
+    /\ is_valid_plaintext2 h0 p2
+    /\ is_valid_plaintext3 h0 p3
+    /\ live h0 msg3
+
+    // Disjointness
+    /\ handshake_state_m_disjoint_to_party_state hs rs
+    /\ AuxMsg2.handshake_state_m_disjoint_to_p2 hs p2
+    /\ handshake_state_m_disjoint_to_lbuffer hs msg3
+    /\ handshake_state_m_disjoint_to_p3 hs p3
+
+    /\ AuxMsg2.party_state_disjoint_to_p2 rs p2
+    /\ party_state_disjoint_to_p3 rs p3
+    /\ party_state_disjoint_to_lbuffer rs msg3
+
+    /\ plaintext2_disjoint_to_lbuffer p2 msg3
+
+    /\ plaintext3_disjoint_to_plaintex2 p3 p2
+    /\ plaintext3_disjoint_to_lbuffer p3 msg3
+  )
+  (ensures fun h0 res h1 ->
+    let base_modified_locs = lbufferOpt_loc hs.th3 in
+
+    match res with
+      | TypeEdhoc.CUnsupportedAlgorithmOrInvalidConfig
+      | TypeEdhoc.CDecryptionFailure -> (
+        modifies base_modified_locs h0 h1
+        /\ lbufferOpt_is_Some h1 hs.th3
+      )
+      | TypeEdhoc.CIntegrityCheckFailed -> (
+        let modified_locs = base_modified_locs |+| lbufferOpt_loc hs.prk4e3m
+                          |+| plaintext3_union p3 in
+
+        modifies modified_locs h0 h1
+        /\ lbufferOpt_is_Some h1 hs.th3 /\ lbufferOpt_is_Some h1 hs.prk4e3m
+      )
+      | TypeEdhoc.CSuccess -> (
+        let modified_locs = base_modified_locs
+                |+| lbufferOpt_loc hs.prk4e3m
+                |+| plaintext3_union p3
+                |+| lbufferOpt_loc hs.th4 |+| lbufferOpt_loc hs.prk_out
+                |+| lbufferOpt_loc hs.prk_exporter in
+
+        modifies modified_locs h0 h1
+        /\ lbufferOpt_is_Some h1 hs.th3 /\ lbufferOpt_is_Some h1 hs.prk4e3m
+        /\ lbufferOpt_is_Some h1 hs.th4 /\ lbufferOpt_is_Some h1 hs.prk_out
+        /\ lbufferOpt_is_Some h1 hs.prk_exporter
+      )
+      | _ -> False
+  )
+
+#push-options "--z3refresh --z3rlimit 150 --fuel 2 --ifuel 1"
+
+let responder_process_msg3_decrypt_msg3 #kcs rs hs p2 msg3 p3
+  = (**) let h0 = ST.get () in
+  ST.push_frame();
+
+  // derive TH3
+  let cred_R = create (size SpecParser.cred_size) (u8 0) in
+  copy cred_R rs.id_cred;
+  compute_th3 #kcs hs.th2.value p2 cred_R hs.th3.value;
+  lbufferOpt_set_Some hs.th3; // set TH3 as Some
+  (**) let h1 = ST.get () in
+  (**) assert(is_valid_handshake_state_m h1 hs);
+
+  // create plaintext3
+  let p3_buffer = create (plaintext3_size_t kcs) (u8 0) in
+
+  // decrypt ciphertext3
+  let res = decrypt_ciphertext3 #kcs msg3 hs.th3.value hs.prk3e2m.value p3_buffer in
+  (**) let h1_1 = ST.get () in
+
+  let final_res = match res with
+    | TypeEdhoc.CUnsupportedAlgorithmOrInvalidConfig -> (
+      (**) let h2_1 = ST.get () in
+      (**) assert(modifies0 h1_1 h2_1);
+      
+      TypeEdhoc.CUnsupportedAlgorithmOrInvalidConfig
+    )
+    | TypeEdhoc.CDecryptionFailure -> (
+      (**) let h2_1 = ST.get () in
+      (**) assert(modifies0 h1_1 h2_1);
+
+      TypeEdhoc.CDecryptionFailure
+    )
+    | TypeEdhoc.CSuccess -> (
+      (**) let h2_1 = ST.get () in
+      (**) assert(is_valid_handshake_state_m h2_1 hs);
+
+      // deserialize plaintext3
+      deserialize_ptx3 kcs p3_buffer p3;
+      (**) let h2 = ST.get () in
+      (**) assert(
+        modifies (plaintext3_union p3) h1_1 h2
+      );
+
+      // process plaintext3
+      let res_process = responder_process_msg3_decrypt_msg3_uti #kcs rs hs p3 in
+      (**) let h3 = ST.get () in
+      (**) assert(
+        let base_modified_locs = lbufferOpt_loc hs.prk4e3m
+                      |+| plaintext3_union p3 in
+
+        match res_process with
+          | TypeEdhoc.CIntegrityCheckFailed -> (
+
+            modifies base_modified_locs h2_1 h3
+            /\ lbufferOpt_is_Some h3 hs.prk4e3m
+          )
+          | TypeEdhoc.CSuccess -> (
+            let modified_locs = base_modified_locs
+                |+| lbufferOpt_loc hs.th4 |+| lbufferOpt_loc hs.prk_out
+                |+| lbufferOpt_loc hs.prk_exporter in
+
+            modifies modified_locs h2_1 h3
+            /\ lbufferOpt_is_Some h3 hs.prk4e3m
+            /\ lbufferOpt_is_Some h3 hs.th4 /\ lbufferOpt_is_Some h3 hs.prk_out
+            /\ lbufferOpt_is_Some h3 hs.prk_exporter
+          )
+          | _ -> False
+      );
+
+
+      res_process
+    ) in
+
+  ST.pop_frame();
+  (**) let h_final = ST.get () in
+  (**) assert(
+    let base_modified_locs = lbufferOpt_loc hs.th3 in
+
+    match final_res with
+      | TypeEdhoc.CUnsupportedAlgorithmOrInvalidConfig
+      | TypeEdhoc.CDecryptionFailure -> (
+        modifies base_modified_locs h0 h_final
+        /\ lbufferOpt_is_Some h_final hs.th3
+      )
+      | TypeEdhoc.CIntegrityCheckFailed -> (
+        let modified_locs = base_modified_locs |+| lbufferOpt_loc hs.prk4e3m
+                         |+| plaintext3_union p3 in
+
+        modifies modified_locs h0 h_final
+        /\ lbufferOpt_is_Some h_final hs.th3 /\ lbufferOpt_is_Some h_final hs.prk4e3m
+      )
+      | TypeEdhoc.CSuccess -> (
+        let modified_locs = base_modified_locs
+                |+| lbufferOpt_loc hs.prk4e3m
+                |+| plaintext3_union p3
+                |+| lbufferOpt_loc hs.th4 |+| lbufferOpt_loc hs.prk_out
+                |+| lbufferOpt_loc hs.prk_exporter in
+
+        modifies modified_locs h0 h_final
+        /\ lbufferOpt_is_Some h_final hs.th3 /\ lbufferOpt_is_Some h_final hs.prk4e3m
+        /\ lbufferOpt_is_Some h_final hs.th4 /\ lbufferOpt_is_Some h_final hs.prk_out
+        /\ lbufferOpt_is_Some h_final hs.prk_exporter
+      )
+      | _ -> False
+  );
+  final_res
+
+#pop-options
