src/kemedhoc/Impl.KEMEDHOC.Core.Msg3.Aux.fst
@@ -1,0 +1,488 @@
+module Impl.KEMEDHOC.Core.Msg3.Aux
+
+(*LowStar related modules*)
+open Lib.ByteBuffer
+open Lib.IntTypes
+open Lib.Buffer
+
+(*HACL Random lib*)
+open Lib.RandomBuffer.System
+module HACLRandom = Lib.RandomSequence
+
+module B = LowStar.Buffer
+module ST = FStar.HyperStack.ST
+module HS = FStar.HyperStack
+module S = FStar.Seq
+module Seq = Lib.Sequence
+
+(*Specification modules*)
+module Spec = Spec.KEMEDHOC.Core
+
+module FBytes = FStar.Bytes
+
+module SpecCrypto = Spec.KEMEDHOC.CryptoPrimitives
+module SpecParser = Spec.KEMEDHOC.Parser
+module SpecTH = Spec.KEMEDHOC.TranscriptHash
+module SpecKS = Spec.KEMEDHOC.KeySchedule
+
+module SpecEdhocSerd = Spec.EDHOC.Serialization
+
+module TypeEdhoc = TypeHelper.EDHOC
+
+(*EDHOC utilities*)
+open Impl.EDHOC.Utilities
+
+(*KEMEDHOC utilities*)
+open Impl.KEMEDHOC.Types
+open Impl.KEMEDHOC.CryptoPrimitives
+open Impl.KEMEDHOC.KeySchedule
+open Impl.KEMEDHOC.Parser
+open Impl.KEMEDHOC.Ciphertext
+open Impl.KEMEDHOC.TranscriptHash
+open Impl.KEMEDHOC.Core
+open Impl.KEMEDHOC.Core.Utilities
+open Spec.KEMEDHOC.Base.Definitions
+
+module AuxMsg2 = Impl.KEMEDHOC.Core.Msg2.Aux
+
+(*------------------ Utilities*)
+/// Should be moved later to a separate module
+let handshake_state_m_disjoint_to_p3 (#kcs: supportedKemCipherSuite)
+  (hs: handshake_state_m kcs) (p3: plaintext3 kcs)
+  = B.all_disjoint [
+    // handshake_state fields
+    loc hs.suite_i; loc hs.msg1_hash;
+    loc hs.k_xy.is_some; loc hs.k_xy.value;
+    loc hs.k_auth_R;
+    loc hs.k_auth_I.is_some; loc hs.k_auth_I.value;
+    loc hs.th1;
+    loc hs.th2.is_some; loc hs.th2.value;
+    loc hs.th3.is_some; loc hs.th3.value;
+    loc hs.th4.is_some; loc hs.th4.value;
+    loc hs.prk1e;
+    loc hs.prk2e.is_some; loc hs.prk2e.value;
+    loc hs.prk3e2m.is_some; loc hs.prk3e2m.value;
+    loc hs.prk4e3m.is_some; loc hs.prk4e3m.value;
+    loc hs.prk_out.is_some; loc hs.prk_out.value;
+    loc hs.prk_exporter.is_some; loc hs.prk_exporter.value;
+    loc hs.remote_id_cred.is_some; loc hs.remote_id_cred.value;
+
+    // plaintext3 fields
+    loc p3.id_cred_I; loc p3.mac3
+  ]
+
+let party_state_disjoint_to_p3 (#kcs: supportedKemCipherSuite)
+  (ps: party_state_m kcs) (p3: plaintext3 kcs)
+  = B.all_disjoint [
+    // party_state fields
+    loc ps.suite; loc (fst ps.static_kem_kp);
+    loc (snd ps.static_kem_kp);
+    loc ps.id_cred;
+    loc ps.eph_kem_priv_key.is_some; loc ps.eph_kem_priv_key.value;
+    loc ps.remote_static_kem_pub_key; loc ps.remote_id_cred;
+
+    // plaintext3 fields
+    loc p3.id_cred_I; loc p3.mac3
+  ]
+
+let plaintext3_disjoint_to_plaintex2 (#kcs: supportedKemCipherSuite)
+  (p3: plaintext3 kcs) (p2: plaintext2 kcs)
+  = B.all_disjoint [
+    // plaintext3 fields
+    loc p3.id_cred_I; loc p3.mac3;
+
+    // plaintext 2 fields
+    loc p2.c_R; loc p2.id_cred_R;
+    loc p2.cred_R; loc p2.mac2
+  ]
+
+(*------------------ Responder's side*)
+
+
+#push-options "--z3refresh --z3rlimit 200 --max_fuel 2 --max_ifuel 1"
+
+let responder_process_msg3_check_mac3 (#kcs: supportedKemCipherSuite)
+  (rs: party_state_m kcs) (hs: handshake_state_m kcs)
+  (p3: plaintext3 kcs) (mac3_buff: mac23_buff kcs) (cred_I: cred_buffer)
+  : ST.Stack c_response
+  (ensures fun h0 ->
+    is_valid_handshake_state_m h0 hs
+    /\ is_valid_party_state_m h0 rs
+    /\ is_valid_plaintext3 h0 p3
+    /\ live h0 mac3_buff /\ live h0 cred_I
+
+    // /\ lbufferOpt_is_Some h0 hs.th3
+    // /\ lbufferOpt_is_Some h0 hs.prk4e3m
+
+    // Disjointness
+    /\ handshake_state_m_disjoint_to_party_state hs rs
+    /\ handshake_state_m_disjoint_to_p3 hs p3
+    /\ handshake_state_m_disjoint_to_lbuffer hs mac3_buff
+    /\ party_state_disjoint_to_p3 rs p3
+    /\ party_state_disjoint_to_lbuffer rs mac3_buff
+    /\ plaintext3_disjoint_to_lbuffer p3 mac3_buff
+    /\ handshake_state_m_disjoint_to_lbuffer hs cred_I
+    /\ party_state_disjoint_to_lbuffer rs cred_I
+    /\ plaintext3_disjoint_to_lbuffer p3 cred_I
+    /\ disjoint mac3_buff cred_I
+  )
+  (requires fun h0 res h1 ->
+    let modified_locs = lbufferOpt_loc hs.th4 |+| lbufferOpt_loc hs.prk_out
+              |+| lbufferOpt_loc hs.prk_exporter in
+
+    (match res with
+      | TypeEdhoc.CIntegrityCheckFailed -> modifies0 h0 h1
+      | TypeEdhoc.CSuccess -> (
+        modifies modified_locs h0 h1
+        /\ lbufferOpt_is_Some h1 hs.th4 /\ lbufferOpt_is_Some h1 hs.prk_out
+        /\ lbufferOpt_is_Some h1 hs.prk_exporter
+      )
+      | _ -> False
+    )
+    /\ is_valid_handshake_state_m h1 hs
+    /\ is_valid_party_state_m h1 rs
+    /\ is_valid_plaintext3 h1 p3
+  )
+  = (**) let h0 = ST.get () in
+
+  let final_res = match (check_mac mac3_buff p3.mac3) with
+    | TypeEdhoc.CIntegrityCheckFailed -> TypeEdhoc.CIntegrityCheckFailed
+    | TypeEdhoc.CSuccess -> (
+      // compute th4
+      compute_th4 #kcs hs.th3.value p3 cred_I hs.th4.value;
+      lbufferOpt_set_Some hs.th4; // set TH4 as Some
+
+      // derive PRK_OUT
+      expand_prk_out #kcs hs.prk4e3m.value hs.th4.value hs.prk_out.value;
+      lbufferOpt_set_Some hs.prk_out; // set PRK_OUT as Some
+
+      // derive PRK_EXPORTER
+      expand_prk_exporter #kcs hs.prk_out.value hs.prk_exporter.value;
+      lbufferOpt_set_Some hs.prk_exporter; // set PRK_EXPORTER as Some
+
+      TypeEdhoc.CSuccess
+    ) in
+
+  (**) let h_final = ST.get () in
+  final_res
+
+
+val responder_process_msg3_decrypt_msg3_uti:
+  #kcs: supportedKemCipherSuite
+  -> rs: party_state_m kcs
+  -> hs: handshake_state_m kcs
+  -> p3: plaintext3 kcs
+  -> ST.Stack c_response
+  (requires fun h0 ->
+    is_valid_handshake_state_m h0 hs
+    /\ is_valid_party_state_m h0 rs
+    /\ is_valid_plaintext3 h0 p3
+
+    // /\ lbufferOpt_is_Some h0 hs.k_auth_I
+    // /\ lbufferOpt_is_Some h0 hs.th3
+
+    // Disjointness
+    /\ handshake_state_m_disjoint_to_party_state hs rs
+    /\ handshake_state_m_disjoint_to_p3 hs p3
+    /\ party_state_disjoint_to_p3 rs p3
+  )
+  (ensures fun h0 res h1 ->
+    let base_modified_locs = lbufferOpt_loc hs.prk4e3m in
+
+    // True
+    (match res with
+      | TypeEdhoc.CIntegrityCheckFailed -> (
+        modifies base_modified_locs h0 h1
+        /\ lbufferOpt_is_Some h1 hs.prk4e3m
+      )
+      | TypeEdhoc.CSuccess -> (
+        let modified_locs = base_modified_locs
+                |+| lbufferOpt_loc hs.th4 |+| lbufferOpt_loc hs.prk_out
+                |+| lbufferOpt_loc hs.prk_exporter in
+
+        modifies modified_locs h0 h1
+        /\ lbufferOpt_is_Some h1 hs.prk4e3m
+        /\ lbufferOpt_is_Some h1 hs.th4 /\ lbufferOpt_is_Some h1 hs.prk_out
+        /\ lbufferOpt_is_Some h1 hs.prk_exporter
+      )
+      | _ -> False
+    )
+  )
+
+
+let responder_process_msg3_decrypt_msg3_uti #kcs rs hs p3
+  = (**) let h0 = ST.get () in
+  ST.push_frame();
+
+  // derive salt4e3m
+  let salt4e3m = create (hash_size_t kcs) (u8 0) in
+  expand_salt #kcs SpecKS.info_label_salt4e3m hs.prk3e2m.value hs.th3.value salt4e3m;
+  (**) let h1 = ST.get () in
+
+  // derive PRK4e3m
+  extract_prk4e3m #kcs salt4e3m hs.k_auth_I.value hs.prk4e3m.value;
+  lbufferOpt_set_Some hs.prk4e3m; // set PRK4e3m as Some
+  (**) let h2 = ST.get () in
+  (**) assert(
+    lbufferOpt_is_Some h2 hs.prk4e3m
+    /\ modifies (lbufferOpt_loc hs.prk4e3m) h1 h2
+  );
+
+  // construct context3
+  let cred_I = create (size SpecParser.cred_size) (u8 0) in
+  copy cred_I p3.id_cred_I;
+
+  let ctx3: context3 kcs = {
+    id_cred_i = p3.id_cred_I;
+    th3 = hs.th3.value;
+    cred_i = cred_I;
+  } in
+  
+  // derive MAC3
+  let mac3 = create (size (SpecCrypto.mac23_size kcs)) (u8 0) in
+  expand_mac3 #kcs hs.prk4e3m.value ctx3 mac3;
+  (**) let h3 = ST.get () in
+  (**) assert(
+    is_valid_handshake_state_m h3 hs
+    /\ is_valid_party_state_m h3 rs
+    /\ is_valid_plaintext3 h3 p3
+    /\ live h3 mac3 /\ live h3 cred_I
+
+    // /\ lbufferOpt_is_Some h3 hs.th3
+    // /\ lbufferOpt_is_Some h3 hs.prk4e3m
+
+    // Disjointness
+    /\ handshake_state_m_disjoint_to_party_state hs rs
+    /\ handshake_state_m_disjoint_to_p3 hs p3
+    /\ handshake_state_m_disjoint_to_lbuffer hs mac3
+    /\ party_state_disjoint_to_p3 rs p3
+    /\ party_state_disjoint_to_lbuffer rs mac3
+    /\ plaintext3_disjoint_to_lbuffer p3 mac3
+    /\ handshake_state_m_disjoint_to_lbuffer hs cred_I
+    /\ party_state_disjoint_to_lbuffer rs cred_I
+    /\ plaintext3_disjoint_to_lbuffer p3 cred_I
+    /\ disjoint mac3 cred_I
+  );
+
+  // check MAC3
+  let final_res = responder_process_msg3_check_mac3 #kcs rs hs p3 mac3 cred_I in
+  (**) let h4 = ST.get () in
+  (**) assert(
+    match final_res with
+      | TypeEdhoc.CIntegrityCheckFailed -> modifies0 h3 h4
+      | TypeEdhoc.CSuccess -> (
+        modifies (lbufferOpt_loc hs.th4 |+| lbufferOpt_loc hs.prk_out
+                |+| lbufferOpt_loc hs.prk_exporter) h3 h4
+        
+        /\ lbufferOpt_is_Some h4 hs.th4
+        /\ lbufferOpt_is_Some h4 hs.prk_out
+        /\ lbufferOpt_is_Some h4 hs.prk_exporter
+      )
+      | _ -> False
+  );
+
+  ST.pop_frame();
+  (**) let h_final = ST.get () in
+  (**) assert(
+    match final_res with
+      | TypeEdhoc.CIntegrityCheckFailed -> (
+        modifies (lbufferOpt_loc hs.prk4e3m) h0 h_final
+        /\ lbufferOpt_is_Some h_final hs.prk4e3m
+      )
+      | TypeEdhoc.CSuccess -> (
+        let modified_locs = (lbufferOpt_loc hs.prk4e3m)
+                |+| lbufferOpt_loc hs.th4 |+| lbufferOpt_loc hs.prk_out
+                |+| lbufferOpt_loc hs.prk_exporter in
+
+        modifies modified_locs h0 h_final
+        /\ lbufferOpt_is_Some h_final hs.prk4e3m
+        /\ lbufferOpt_is_Some h_final hs.th4 /\ lbufferOpt_is_Some h_final hs.prk_out
+        /\ lbufferOpt_is_Some h_final hs.prk_exporter
+      )
+  );
+
+  final_res
+
+
+#pop-options
+
+
+(*------------------ Initiator's side*)
+
+val initiator_send_msg3_construct_msg3:
+  #kcs: supportedKemCipherSuite
+  -> is: party_state_m kcs
+  -> hs: handshake_state_m kcs
+  -> msg3: message3 kcs
+  -> ST.Stack c_response
+  (requires fun h0 ->
+    is_valid_handshake_state_m h0 hs
+    /\ is_party_state_eph_est_m h0 is
+    // /\ is_valid_handshake_state_m_after_msg2 h0 hs
+    /\ live h0 msg3
+
+    /\ lbufferOpt_is_Some h0 hs.prk4e3m /\ lbufferOpt_is_Some h0 hs.th3
+
+    // Disjointness
+    /\ handshake_state_m_disjoint_to_party_state hs is
+    /\ handshake_state_m_disjoint_to_lbuffer hs msg3
+    /\ party_state_disjoint_to_lbuffer is msg3
+  )
+  (ensures fun h0 res h1 ->
+    match res with
+      | TypeEdhoc.CUnsupportedAlgorithmOrInvalidConfig -> modifies0 h0 h1
+      | TypeEdhoc.CSuccess -> (
+        let modified_locs = lbufferOpt_loc hs.th4 |+| lbufferOpt_loc hs.prk_out
+                  |+| lbufferOpt_loc hs.prk_exporter
+                  |+| loc msg3 in
+
+        modifies modified_locs h0 h1
+        /\ lbufferOpt_is_Some h1 hs.th4 /\ lbufferOpt_is_Some h1 hs.prk_out
+        /\ lbufferOpt_is_Some h1 hs.prk_exporter
+        // /\ is_valid_handshake_state_m_after_msg3 h1 hs
+      )
+      | _ -> False
+  )
+
+#push-options "--z3refresh --z3rlimit 50 --max_fuel 2 --max_ifuel 2"
+let initiator_send_msg3_construct_msg3 #kcs is hs msg3
+  = (**) let h0 = ST.get () in
+  ST.push_frame();
+
+  // create a buffer for credential R payload
+  // in real world, the credential payload should be stored
+  // locally in the communing party.
+  let cred_I = create (size SpecParser.cred_size) (u8 0) in
+  copy cred_I is.id_cred;
+
+  // construct context3
+  let ctx3: context3 kcs = {
+    id_cred_i = is.id_cred;
+    th3 = hs.th3.value;
+    cred_i = cred_I;
+  } in
+
+  // derive MAC3
+  let mac3 = create (size (SpecCrypto.mac23_size kcs)) (u8 0) in
+  expand_mac3 #kcs hs.prk4e3m.value ctx3 mac3;
+
+  // construct plaintext3
+  let p3: plaintext3 kcs = {
+    id_cred_I = is.id_cred;
+    mac3 = mac3;
+  } in
+
+  // encrypt plaintext3
+  let final_res = match (encrypt_plaintext3 #kcs p3 hs.th3.value hs.prk3e2m.value msg3) with
+    | TypeEdhoc.CUnsupportedAlgorithmOrInvalidConfig -> TypeEdhoc.CUnsupportedAlgorithmOrInvalidConfig
+    | TypeEdhoc.CSuccess -> (
+      // compute TH4
+      compute_th4 #kcs hs.th3.value p3 cred_I hs.th4.value;
+      lbufferOpt_set_Some hs.th4; // set TH4 as Some
+
+      // derive PRK_OUT
+      expand_prk_out #kcs hs.prk4e3m.value hs.th4.value hs.prk_out.value;
+      lbufferOpt_set_Some hs.prk_out; // set PRK_OUT as Some
+
+      // derive PRK_EXPORTER
+      expand_prk_exporter #kcs hs.prk_out.value hs.prk_exporter.value;
+      lbufferOpt_set_Some hs.prk_exporter; // set PRK_EXPORTER as Some
+
+      TypeEdhoc.CSuccess
+    ) in
+
+
+  ST.pop_frame();
+  (**) let h_final = ST.get () in
+  (**) assert(
+    match final_res with
+      | TypeEdhoc.CUnsupportedAlgorithmOrInvalidConfig -> modifies0 h0 h_final
+      | TypeEdhoc.CSuccess -> (
+        let modified_locs = lbufferOpt_loc hs.th4 |+| lbufferOpt_loc hs.prk_out
+                  |+| lbufferOpt_loc hs.prk_exporter
+                  |+| loc msg3 in
+
+        modifies modified_locs h0 h_final
+        /\ lbufferOpt_is_Some h_final hs.th4 /\ lbufferOpt_is_Some h_final hs.prk_out
+        /\ lbufferOpt_is_Some h_final hs.prk_exporter
+        // /\ is_valid_handshake_state_m_after_msg3 h_final hs
+      )
+  );
+
+  final_res
+
+#pop-options
+
+
+val initiator_send_msg3_set_up:
+  #kcs: supportedKemCipherSuite
+  -> is: party_state_m kcs
+  -> hs: handshake_state_m kcs
+  -> p2: plaintext2 kcs
+  -> ST.Stack unit
+  (requires fun h0 ->
+    is_party_state_eph_est_m h0 is
+    /\ is_valid_handshake_state_m h0 hs
+    // /\ is_valid_handshake_state_m_after_msg2 h0 hs
+    /\ is_valid_plaintext2 h0 p2
+
+    /\ lbufferOpt_is_Some h0 hs.th2 /\ lbufferOpt_is_Some h0 hs.prk3e2m
+    /\ lbufferOpt_is_Some h0 hs.k_auth_I
+
+    // Disjointness
+    /\ handshake_state_m_disjoint_to_party_state hs is
+    /\ AuxMsg2.handshake_state_m_disjoint_to_p2 hs p2
+    /\ AuxMsg2.party_state_disjoint_to_p2 is p2
+  )
+  (ensures fun h0 _ h1 ->
+    let modified_locs = lbufferOpt_loc hs.th3 |+| lbufferOpt_loc hs.prk4e3m in
+
+    modifies modified_locs h0 h1
+    // As the two below fields are Some, directly conflicts the post-condition
+    // `is_valid_handshake_state_m_after_msg2` where the two fields should
+    // be None.
+    /\ lbufferOpt_is_Some h1 hs.th3 /\ lbufferOpt_is_Some h1 hs.prk4e3m
+    /\ is_valid_handshake_state_m h1 hs
+    /\ is_party_state_eph_est_m h1 is
+    /\ is_valid_plaintext2 h1 p2
+  )
+
+#push-options "--z3refresh --z3rlimit 80 --max_fuel 2 --max_ifuel 2"
+let initiator_send_msg3_set_up #kcs is hs p2
+  = (**) let h0 = ST.get () in
+  ST.push_frame();
+  
+  // create a buffer for credential R payload
+  // in real world, the credential payload should be stored
+  // locally in the communing party.
+  let cred_R = create (size SpecParser.cred_size) (u8 0) in
+  copy cred_R p2.id_cred_R;
+
+  // derive TH3
+  compute_th3 #kcs hs.th2.value p2 cred_R hs.th3.value;
+  lbufferOpt_set_Some hs.th3; // set TH3 as Some
+
+  // derive SALT4e3m
+  let salt4e3m = create (hash_size_t kcs) (u8 0) in
+  expand_salt #kcs SpecKS.info_label_salt4e3m hs.prk3e2m.value hs.th3.value salt4e3m;
+
+  // derive PRK4e3m
+  extract_prk4e3m #kcs salt4e3m hs.k_auth_I.value hs.prk4e3m.value;
+  lbufferOpt_set_Some hs.prk4e3m; // set PRK4e3m as Some
+
+  ST.pop_frame();
+  (**) let h_final =  ST.get() in
+  (**) assert(
+    let modified_locs = lbufferOpt_loc hs.th3 |+| lbufferOpt_loc hs.prk4e3m in
+
+    modifies modified_locs h0 h_final
+    // As the two below fields are Some, directly conflicts the post-condition
+    // `is_valid_handshake_state_m_after_msg2` where the two fields should
+    // be None.
+    /\ lbufferOpt_is_Some h_final hs.th3 /\ lbufferOpt_is_Some h_final hs.prk4e3m
+    /\ is_valid_handshake_state_m h_final hs
+    /\ is_party_state_eph_est_m h_final is
+    /\ is_valid_plaintext2 h_final p2
+  )
+
+#pop-options
