src/kemedhoc/Impl.KEMEDHOC.Core.Msg3.fst
@@ -1,0 +1,80 @@
+module Impl.KEMEDHOC.Core.Msg3
+
+module HACLRandom = Lib.RandomSequence
+
+module B = LowStar.Buffer
+module ST = FStar.HyperStack.ST
+module HS = FStar.HyperStack
+module S = FStar.Seq
+module Seq = Lib.Sequence
+
+(*Specification modules*)
+module Spec = Spec.KEMEDHOC.Core
+
+module SpecCrypto = Spec.KEMEDHOC.CryptoPrimitives
+module SpecParser = Spec.KEMEDHOC.Parser
+module SpecTH = Spec.KEMEDHOC.TranscriptHash
+module SpecKS = Spec.KEMEDHOC.KeySchedule
+
+module SpecEdhocSerd = Spec.EDHOC.Serialization
+
+module TypeEdhoc = TypeHelper.EDHOC
+
+#push-options "--z3refresh --z3rlimit 70 --max_fuel 2 --max_ifuel 1"
+
+(*------------------ Responder's side*)
+let responder_process_msg3 kcs rs hs p2 msg3 p3
+  = (**) let h0 = ST.get() in
+
+  (**) assert(is_valid_handshake_state_m h0 hs);
+  let res = responder_process_msg3_decrypt_msg3 #kcs rs hs p2 msg3 p3 in
+  (**) let h_final = ST.get() in
+  (**) assume(
+    let res_s = Spec.responder_process_msg3 kcs (party_state_m_eval h0 rs)
+                (handshake_state_m_eval h0 hs)
+                (plaintext2_eval h0 p2)
+                (as_seq h0 msg3) in
+
+    let hs_s_final = handshake_state_m_eval h_final hs in
+    let p3_s_final = plaintext3_eval h_final p3 in
+
+    match res_s with
+      | Fail e -> res == error_to_c_response e
+      | Res (hs_s, p3_s) -> (
+        res == TypeEdhoc.CSuccess
+        /\ Spec.is_valid_handshake_state_after_msg3 hs_s_final
+        /\ Spec.hs_equal hs_s_final hs_s
+        /\ SpecParser.plaintext3_equal p3_s_final p3_s
+      )
+  );
+  res
+
+(*------------------ Initiator's side*)
+let initiator_send_msg3 kcs is hs p2 msg3
+  = (**) let h0 = ST.get() in
+
+  initiator_send_msg3_set_up #kcs is hs p2;
+  let final_res = initiator_send_msg3_construct_msg3 #kcs is hs msg3 in
+
+
+  (**) let h_final = ST.get() in
+  (**) assume(
+    let res_s = Spec.initiator_send_msg3 kcs (party_state_m_eval h0 is)
+                (handshake_state_m_eval h0 hs)
+                (plaintext2_eval h0 p2) in
+
+    let hs_s_final = handshake_state_m_eval h_final hs in
+    let msg3_s_final = as_seq h_final msg3 in
+
+    match res_s with
+      | Fail e -> final_res == error_to_c_response e
+      | Res (msg3_s, hs_s) -> (
+        final_res == TypeEdhoc.CSuccess
+        /\ Spec.is_valid_handshake_state_after_msg3 hs_s_final
+        /\ Spec.hs_equal hs_s_final hs_s
+        /\ Seq.equal msg3_s_final msg3_s
+      )
+  );
+  final_res
+
+#pop-options
