src/kemedhoc/Impl.KEMEDHOC.Core.Msg3.fsti
@@ -1,0 +1,199 @@
+module Impl.KEMEDHOC.Core.Msg3
+
+(*LowStar related modules*)
+open Lib.ByteBuffer
+open Lib.IntTypes
+open Lib.Buffer
+
+(*HACL Random lib*)
+open Lib.RandomBuffer.System
+module HACLRandom = Lib.RandomSequence
+
+module B = LowStar.Buffer
+module ST = FStar.HyperStack.ST
+module HS = FStar.HyperStack
+module S = FStar.Seq
+module Seq = Lib.Sequence
+
+(*Specification modules*)
+module Spec = Spec.KEMEDHOC.Core
+
+module SpecCrypto = Spec.KEMEDHOC.CryptoPrimitives
+module SpecParser = Spec.KEMEDHOC.Parser
+module SpecTH = Spec.KEMEDHOC.TranscriptHash
+module SpecKS = Spec.KEMEDHOC.KeySchedule
+
+module SpecEdhocSerd = Spec.EDHOC.Serialization
+
+module TypeEdhoc = TypeHelper.EDHOC
+
+(*EDHOC utilities*)
+open Impl.EDHOC.Utilities
+
+(*KEMEDHOC utilities*)
+open Impl.KEMEDHOC.Types
+open Impl.KEMEDHOC.CryptoPrimitives
+open Impl.KEMEDHOC.KeySchedule
+open Impl.KEMEDHOC.Parser
+open Impl.KEMEDHOC.Ciphertext
+open Impl.KEMEDHOC.TranscriptHash
+open Impl.KEMEDHOC.Core
+open Spec.KEMEDHOC.Base.Definitions
+
+open Impl.KEMEDHOC.Core.Msg3.Aux
+open Impl.KEMEDHOC.Core.Msg3.Aux.Misc
+module AuxMsg2 = Impl.KEMEDHOC.Core.Msg2.Aux
+
+(*------------------ Utilities*)
+
+(*------------------ Responder's side*)
+val responder_process_msg3:
+  kcs: supportedKemCipherSuite
+  -> rs: party_state_m kcs
+  -> hs: handshake_state_m kcs
+  -> p2: plaintext2 kcs
+  -> msg3: message3 kcs
+  -> p3: plaintext3 kcs
+  -> ST.Stack c_response
+  (requires fun h0 ->
+    is_party_state_eph_est_m h0 rs
+    
+    /\ is_valid_handshake_state_m h0 hs
+    /\ is_valid_handshake_state_m_after_msg2 h0 hs
+    /\ lbufferOpt_is_Some h0 hs.remote_id_cred
+
+    /\ is_valid_plaintext2 h0 p2
+    /\ is_valid_plaintext3 h0 p3
+    /\ live h0 msg3
+
+    // Disjointness
+    /\ handshake_state_m_disjoint_to_party_state hs rs
+    /\ AuxMsg2.handshake_state_m_disjoint_to_p2 hs p2
+    /\ handshake_state_m_disjoint_to_lbuffer hs msg3
+    /\ handshake_state_m_disjoint_to_p3 hs p3
+
+    /\ AuxMsg2.party_state_disjoint_to_p2 rs p2
+    /\ party_state_disjoint_to_p3 rs p3
+    /\ party_state_disjoint_to_lbuffer rs msg3
+
+    /\ plaintext2_disjoint_to_lbuffer p2 msg3
+
+    /\ plaintext3_disjoint_to_plaintex2 p3 p2
+    /\ plaintext3_disjoint_to_lbuffer p3 msg3
+  )
+  (ensures fun h0 res h1 ->
+    let base_modified_locs = lbufferOpt_loc hs.th3 in
+
+    is_party_state_eph_est_m h1 rs
+    /\ is_valid_handshake_state_m h1 hs
+    // Memory modification and validity of the handshake state
+    /\ (match res with
+      | TypeEdhoc.CUnsupportedAlgorithmOrInvalidConfig
+      | TypeEdhoc.CDecryptionFailure -> (
+        modifies base_modified_locs h0 h1
+        /\ lbufferOpt_is_Some h1 hs.th3
+      )
+      | TypeEdhoc.CIntegrityCheckFailed -> (
+        let modified_locs = base_modified_locs |+| lbufferOpt_loc hs.prk4e3m
+                          |+| plaintext3_union p3 in
+
+        modifies modified_locs h0 h1
+        /\ lbufferOpt_is_Some h1 hs.th3 /\ lbufferOpt_is_Some h1 hs.prk4e3m
+      )
+      | TypeEdhoc.CSuccess -> (
+        let modified_locs = base_modified_locs
+                |+| lbufferOpt_loc hs.prk4e3m
+                |+| plaintext3_union p3
+                |+| lbufferOpt_loc hs.th4 |+| lbufferOpt_loc hs.prk_out
+                |+| lbufferOpt_loc hs.prk_exporter in
+
+        modifies modified_locs h0 h1
+        /\ is_valid_handshake_state_m_after_msg3 h1 hs
+      )
+      | _ -> False)
+      // Functional correctness w.r.t. the high-level specification
+      /\ (
+        let rs_init = party_state_m_eval h0 rs in
+        let hs_init = handshake_state_m_eval h0 hs in
+        let p2_init = plaintext2_eval h0 p2 in
+        let msg3_init = as_seq h0 msg3 in
+
+        let res_s = Spec.responder_process_msg3 kcs rs_init hs_init p2_init msg3_init in
+        match res_s with
+          | Fail e -> res == error_to_c_response e
+          | Res (hs_s, p3_s) -> (
+            let hs_final = handshake_state_m_eval h1 hs in
+
+            res == TypeEdhoc.CSuccess
+            /\ Spec.is_valid_handshake_state_after_msg3 hs_final
+            /\ Spec.hs_equal hs_s hs_final
+            /\ SpecParser.plaintext3_equal (plaintext3_eval h1 p3) p3_s
+          )
+      )
+  )
+
+(*------------------ Initiator's side*)
+val initiator_send_msg3:
+  kcs: supportedKemCipherSuite
+  -> is: party_state_m kcs
+  -> hs: handshake_state_m kcs
+  -> p2: plaintext2 kcs
+  -> msg3: message3 kcs
+  -> ST.Stack c_response
+  (requires fun h0 ->
+    is_valid_handshake_state_m h0 hs
+    /\ is_valid_handshake_state_m_after_msg2 h0 hs
+    /\ is_valid_party_state_m h0 is
+    /\ is_party_state_eph_est_m h0 is
+    /\ is_valid_plaintext2 h0 p2
+    /\ live h0 msg3
+
+    // Disjointness
+    /\ handshake_state_m_disjoint_to_party_state hs is
+    /\ handshake_state_m_disjoint_to_lbuffer hs msg3
+    /\ AuxMsg2.handshake_state_m_disjoint_to_p2 hs p2
+    /\ AuxMsg2.party_state_disjoint_to_p2 is p2
+    /\ party_state_disjoint_to_lbuffer is msg3
+    /\ plaintext2_disjoint_to_lbuffer p2 msg3
+
+  )
+  (ensures fun h0 res h1 ->
+    let base_modified_locs = lbufferOpt_loc hs.th3 |+| lbufferOpt_loc hs.prk4e3m in
+
+    is_valid_party_state_m h1 is
+    /\ is_party_state_eph_est_m h1 is
+    /\ is_valid_handshake_state_m h1 hs
+    // Memory modification and validity of the handshake state
+    /\ (match res with
+      | TypeEdhoc.CUnsupportedAlgorithmOrInvalidConfig -> (
+        modifies base_modified_locs h0 h1
+      )
+      | TypeEdhoc.CSuccess -> (
+        let modified_locs = base_modified_locs
+                |+| lbufferOpt_loc hs.th4 |+| lbufferOpt_loc hs.prk_out
+                |+| lbufferOpt_loc hs.prk_exporter
+                |+| loc msg3 in
+
+        modifies modified_locs h0 h1
+        /\ is_valid_handshake_state_m_after_msg3 h1 hs
+      )
+      | _ -> False)
+    // Functional correctness w.r.t. the high-level specification
+    /\ (
+      let is_init = party_state_m_eval h0 is in
+      let hs_init = handshake_state_m_eval h0 hs in
+      let p2_init = plaintext2_eval h0 p2 in
+
+      let res_s = Spec.initiator_send_msg3 kcs is_init hs_init p2_init in
+      match res_s with
+        | Fail e -> res == error_to_c_response e
+        | Res (m3_s, hs_s) -> (
+          let hs_final = handshake_state_m_eval h1 hs in
+
+          res == TypeEdhoc.CSuccess
+          /\ Spec.is_valid_handshake_state_after_msg3 hs_final
+          /\ Spec.hs_equal hs_s hs_final
+          /\ Seq.equal (as_seq h1 msg3) m3_s
+        )
+    )
+  )
